refinedVST/typing/malloc.v
@@ -1,7 +1,9 @@
+Set Warnings "-notation-overridden,-custom-entry-overridden,-hiding-delimiting-key".
 From VST.typing Require Export type.
 From VST.typing Require Import programs own.
 From VST.typing Require Import type_options.
 From VST.typing Require Export typing.
+Set Warnings "notation-overridden,custom-entry-overridden,hiding-delimiting-key".
 
 (* TODO: Should this also contain a persistent [malloc_initialized]? *)
 Class mallocG Σ := {
@@ -13,22 +15,22 @@ Section malloc_block.
   Context `{!typeG OK_ty Σ} `{!mallocG Σ}.
 
   Definition FindMallocBlock (l : address) :=
-    {| fic_A := iProp Σ; fic_Prop P := P; |}.
+    {| fic_A := assert; fic_Prop P := P; |}.
   Global Instance related_to_malloc_block A l (n : A → Z) :
-    RelatedTo (λ y : A, malloc_block l (n y)) :=
+    RelatedTo (λ y : A, ⎡malloc_block l (n y)⎤%I) :=
     {| rt_fic := FindMallocBlock l |}.
 
   Lemma find_in_context_malloc_block l T:
     find_in_context (FindMallocBlock l) T :-
-      pattern: n, malloc_block l n; return T (malloc_block l n).
-  Proof. iDestruct 1 as (n) "[Hb HT]". iExists (malloc_block _ _). iFrame. Qed.
+      pattern: n, ⎡malloc_block l n⎤; return T ⎡malloc_block l n⎤.
+  Proof. iDestruct 1 as (n) "[Hb HT]". iExists ⎡malloc_block _ _⎤%I. iFrame. Qed.
   Definition find_in_context_malloc_block_inst :=
     [instance find_in_context_malloc_block with FICSyntactic].
   Global Existing Instance find_in_context_malloc_block_inst | 1.
 
-  Lemma subsume_malloc_block A l n1 n2 T:
-    (∃ x, <affine> ⌜n1 = n2 x⌝ ∗ T x)
-    ⊢ subsume (malloc_block l n1) (λ x : A, malloc_block l (n2 x)) T.
+  Lemma subsume_malloc_block A l n1 n2 (T : A -> assert) :
+    (∃ x : A, <affine> ⌜n1 = n2 x⌝ ∗ T x)
+    ⊢ subsume ⎡malloc_block l n1⎤ (λ x : A, ⎡malloc_block l (n2 x)⎤) T.
   Proof. iIntros "[% [-> ?]] ?". iExists _. iFrame. Qed.
   Definition subsume_malloc_block_inst := [instance subsume_malloc_block].
   Global Existing Instance subsume_malloc_block_inst.
@@ -41,28 +43,28 @@ Section malloced.
   or after ty. This is important for instantiating existentials *)
   Program Definition malloced_gen (early : bool) (n : Z) (ty : type) : type := {|
     ty_has_op_type ot mt := False%type;
-    ty_own β l := (if β is Own then l ◁ₗ{β} ty ∗ malloc_block l n else True)%I;
+    ty_own β l := (if β is Own then l ◁ₗ{β} ty ∗ ⎡malloc_block l n⎤ else True)%I;
     ty_own_val v cty := True%I;
   |}.
   Solve Obligations with try done.
   Next Obligation. by iIntros (??????) "?". Qed.
 
   Lemma simplify_hyp_malloced_gen early l ty n T:
-    (malloc_block l n -∗ l ◁ₗ ty -∗ T) ⊢ simplify_hyp (l ◁ₗ malloced_gen early n ty) T.
+    (⎡malloc_block l n⎤ -∗ l ◁ₗ ty -∗ T) ⊢ simplify_hyp (l ◁ₗ malloced_gen early n ty) T.
   Proof. iIntros "HT [Hl HP]". by iApply ("HT" with "HP"). Qed.
   Definition simplify_hyp_malloced_gen_inst :=
     [instance simplify_hyp_malloced_gen with 0%N].
   Global Existing Instance simplify_hyp_malloced_gen_inst.
 
   Lemma simplify_goal_malloced_early l ty n T:
-    malloc_block l n ∗ l ◁ₗ ty ∗ T  ⊢ simplify_goal (l ◁ₗ malloced_gen true n ty) T.
+    ⎡malloc_block l n⎤ ∗ l ◁ₗ ty ∗ T  ⊢ simplify_goal (l ◁ₗ malloced_gen true n ty) T.
   Proof. by iIntros "[$ [$ $]] !>". Qed.
   Definition simplify_goal_malloced_early_inst :=
     [instance simplify_goal_malloced_early with 0%N].
   Global Existing Instance simplify_goal_malloced_early_inst.
 
   Lemma simplify_goal_malloced_late l ty n T:
-    l ◁ₗ ty ∗ malloc_block l n ∗ T  ⊢ simplify_goal (l ◁ₗ malloced_gen false n ty) T.
+    l ◁ₗ ty ∗ ⎡malloc_block l n⎤ ∗ T  ⊢ simplify_goal (l ◁ₗ malloced_gen false n ty) T.
   Proof. by iIntros "[$ [$ $]] !>". Qed.
   Definition simplify_goal_malloced_late_inst :=
     [instance simplify_goal_malloced_late with 0%N].
